cpu_models/x86model/Model/X86BG.v
@@ -9,9 +9,9 @@ Require Import Coq.Strings.Ascii.
 Require Import Coq.Strings.String.
 Require Import Coq.Program.Program.
 
-Require Import Coqlib.
+Require Import RSCoqlib.
 Require Import CommonTacs.
-Require Import Shared.Maps.
+Require Import Shared.RSMaps.
 
 Unset Automatic Introduction.
 Set Implicit Arguments.
@@ -2219,7 +2219,7 @@ Set Implicit Arguments.
 
   (** Starting constructing the x86 parser *)
   Require Import Parser.
-  Require Import Grammar.
+  Require Import RSGrammar.
 
   Definition instr_regexp :=
     projT1 (split_grammar (bigrammar_to_grammar (proj1_sig instr_bigrammar))).
